finish quicksort example

Iris/Iris/HeapLang/Lib/Quicksort.lean
@@ -11,11 +11,35 @@ open BI Iris ProgramLogic
 
 namespace Quicksort
 
-def cons : Val := hl_val% λ x, injr(ref(x))
+def cons : Val := hl_val% λ x, some(ref(x))
 
-def append : Val := hl_val% rec append f := ref(#false)
+def append : Val := hl_val%
+  rec append x :=
+    let l1 := fst(x);
+    let l2 := snd(x);
+    match l1 with
+    | none() => l2
+    | some(x) =>
+      (let p := !x;
+       let head := fst(p);
+       let tail := snd(p);
+       ?cons (head, append (tail, l2)))
 
-def partition : Val := hl_val% rec append f := ref(#false)
+def partition : Val := hl_val%
+  rec partition arg :=
+    let x := fst(arg);
+    let l := snd(arg);
+    match l with
+    | none() => (none(), none())
+    | some(lx) =>
+      (let p := !lx;
+       let head := fst(p);
+       let tail := snd(p);
+       let part := partition (x, tail);
+       if head ≤ x then
+        (?cons (head, fst(part)), snd(part))
+       else
+        (fst(part), ?cons (head, snd(part))))
 
 def quicksort : Val := hl_val%
   rec quicksort l :=
@@ -51,9 +75,7 @@ theorem cons_spec x l ls Φ :
     (∀ v, isList v (x :: ls) -∗ Φ v) -∗
     WP hl(?cons v((#x, ?l))) {{ Φ }} := by
   iintro Hl HΦ
-  iapply wp_rec; rfl; simp [Exp.subst, Exp.substStr]
-  imodintro
-  wp_pures
+  wp_rec
   wp_bind ref(_)
   iapply wp_alloc
   iintro !> %l Hl
@@ -70,7 +92,31 @@ theorem append_spec l1 ls1 l2 ls2 Φ :
     isList l2 ls2 -∗
     (∀ v, isList v (ls1 ++ ls2) -∗ Φ v) -∗
     WP hl(?append v((?l1, ?l2))) {{ Φ }} := by
-  sorry
+  iintro Hl1 Hl2 HΦ
+  iloeb as IH generalizing %l1 %ls1 %Φ
+  wp_rec
+  rw (occs:=[3]) [isList.eq_def]
+  cases ls1 with
+  | nil =>
+    simp only
+    icases Hl1 with %hl1; subst hl1
+    wp_pures; imodintro; simp
+    iapply HΦ $$ [$]
+  | cons x ls1 =>
+    simp only
+    icases Hl1 with ⟨%x, %tl, %hl1, Hpt, Hl1⟩; subst hl1
+    wp_pures
+    wp_bind !_
+    iapply wp_load $$ [$]
+    iintro !> Hpt
+    wp_pures
+    wp_bind ?append _
+    iapply IH $$ Hl1 Hl2
+    iintro %_ Hl
+    wp_pures
+    iapply cons_spec $$ [$]
+    iintro %_ Hl; simp
+    iapply HΦ $$ [$]
 
 theorem partition_spec x l ls Φ :
     isList (GF:=GF) l ls -∗
@@ -79,7 +125,43 @@ theorem partition_spec x l ls Φ :
       isList l2 (ls.filter (x < ·)) -∗
       Φ hl_val((?l1, ?l2))) -∗
     WP hl(?partition v((#x, ?l))) {{ Φ }} := by
-  sorry
+  iintro Hl HΦ
+  iloeb as IH generalizing %l %ls %Φ
+  wp_rec; wp_pures
+  rw (occs:=[2]) [isList.eq_def]
+  cases ls with
+  | nil =>
+    simp only
+    icases Hl with %hl; subst hl
+    wp_pures; imodintro; simp
+    iapply HΦ <;> simp [isList] <;> itrivial
+  | cons hd ls =>
+    simp only
+    icases Hl with ⟨%_, %tl, %hl, Hpt, Hl⟩; subst hl
+    wp_pures
+    wp_bind !_
+    iapply wp_load $$ [$]
+    iintro !> Hpt
+    wp_pures
+    wp_bind ?partition _
+    iapply IH $$ Hl
+    iintro %l1 %l2 Hl1 Hl2
+    wp_pures
+    by_cases hd ≤ x <;> simp [*] <;> wp_pures
+    all_goals wp_bind ?cons _
+    · iapply cons_spec $$ Hl1
+      iintro %_ _
+      wp_pures
+      imodintro
+      iapply HΦ $$ [$] [$]
+    · iapply cons_spec $$ Hl2
+      iintro %_ _
+      wp_pures
+      imodintro
+      iapply HΦ $$ Hl1
+      have : x < hd := by grind
+      simp [*]
+      iframe
 
 -- set_option profiler true in
 theorem quicksort_spec l ls Φ :
@@ -92,15 +174,14 @@ theorem quicksort_spec l ls Φ :
     WP hl(?quicksort ?l) {{ Φ }} := by
   iintro Hl HΦ
   iloeb as IH generalizing %l %ls %Φ
-  iapply wp_rec; rfl; simp [Exp.subst, Exp.substStr]
-  imodintro
+  wp_rec
   rw (occs:=[2]) [isList.eq_def]
   cases ls with
   | nil =>
     simp
     iclear IH
     icases Hl with %heq; subst heq
-    wp_pures; simp [Exp.subst]
+    wp_pures
     imodintro
     iapply HΦ $$ %_ %([])
     · unfold isList; itrivial
@@ -109,33 +190,26 @@ theorem quicksort_spec l ls Φ :
   | cons head tail =>
     simp
     icases Hl with ⟨%l, %tl, %heq, Hpt, Hl⟩; subst heq
-    wp_pures; simp [Exp.subst, Exp.substStr]
+    wp_pures
     wp_bind !_
     iapply wp_load $$ [$]
     iintro !> Hpt
-    wp_pures; simp [Exp.subst, Exp.substStr]
-    wp_pures; simp [Exp.subst, Exp.substStr]
-    wp_pures; simp [Exp.subst, Exp.substStr]
     wp_pures
     wp_bind ?partition _
     iapply partition_spec $$ [$]
     iintro %l1 %l2 Hl1 Hl2
-    wp_pures; simp [Exp.subst, Exp.substStr]
     wp_pures
     wp_bind ?quicksort _
     iapply IH $$ [$]
     iintro %l1' %ls1' Hl1 %_ %_
-    wp_pures; simp [Exp.subst, Exp.substStr]
     wp_pures
     wp_bind ?quicksort _
     iapply IH $$ [$]
     iintro %l2' %ls2' Hl2 %_ %_
-    wp_pures; simp [Exp.subst, Exp.substStr]
     wp_pures
     wp_bind ?cons _
     iapply cons_spec $$ Hl2
     iintro %_ _
-    wp_pures; simp [Exp.subst, Exp.substStr]
     wp_pures
     iapply append_spec $$ [$] [$]
     iintro %_ _
