Iris/Iris/HeapLang/ProofMode.lean
@@ -22,6 +22,140 @@ open Lean hiding Expr
 open Meta Elab Tactic Qq
 open Iris.HeapLang Iris.BI
 
+public section wp_expr_simp
+
+@[wp_expr_simp]
+theorem subst_anon {v e} : Exp.subst (.anon) v e = e := rfl
+
+@[wp_expr_simp]
+theorem subst_ofVal {x v v'} : Exp.subst (.named x) v (Exp.ofVal v') = (Exp.ofVal v') := rfl
+
+@[wp_expr_simp]
+theorem subst_var_eq {x v} : Exp.subst (.named x) v (.var x) = (Exp.ofVal v) := by simp [Exp.subst, Exp.substStr]
+
+@[wp_expr_simp]
+theorem subst_var_neq {x y v} : x ≠ y → Exp.subst (.named x) v (.var y) = (.var y) := by simp [Exp.subst, Exp.substStr]
+
+@[wp_expr_simp]
+theorem subst_rec_eq {x f fx e v} :
+  .named x = f ∨ .named x = fx →
+  Exp.subst (.named x) v (.rec_ f fx e) = (.rec_ f fx e) :=
+  by simp [Exp.subst, Exp.substStr]; grind
+
+@[wp_expr_simp]
+theorem subst_rec_neq {x f fx e v} :
+  .named x ≠ f →
+  .named x ≠ fx →
+  Exp.subst (.named x) v (.rec_ f fx e) = (.rec_ f fx $ e.subst (.named x) v) :=
+  by simp [Exp.subst, Exp.substStr]; grind
+
+@[wp_expr_simp]
+theorem subst_app {x v e₁ e₂} :
+  Exp.subst (.named x) v (.app e₁ e₂) = (.app (e₁.subst (.named x) v) (e₂.subst (.named x) v)) :=
+  by simp [Exp.subst, Exp.substStr]
+
+@[wp_expr_simp]
+theorem subst_case {x v e₁ e₂ e₃} :
+  Exp.subst (.named x) v (.case e₁ e₂ e₃) = (.case (e₁.subst (.named x) v) (e₂.subst (.named x) v) (e₃.subst (.named x) v)) :=
+  by simp [Exp.subst, Exp.substStr]
+
+@[wp_expr_simp]
+theorem subst_unop {x v op e} :
+  Exp.subst (.named x) v (.unop op e) = (.unop op (e.subst (.named x) v)) :=
+  by simp [Exp.subst, Exp.substStr]
+
+@[wp_expr_simp]
+theorem subst_binop {x v op e₁ e₂} :
+  Exp.subst (.named x) v (.binop op e₁ e₂) = (.binop op (e₁.subst (.named x) v) (e₂.subst (.named x) v)) :=
+  by simp [Exp.subst, Exp.substStr]
+
+@[wp_expr_simp]
+theorem subst_if {x v e₀ e₁ e₂} :
+  Exp.subst (.named x) v (.if e₀ e₁ e₂) = (.if (e₀.subst (.named x) v) (e₁.subst (.named x) v) (e₂.subst (.named x) v)) :=
+  by simp [Exp.subst, Exp.substStr]
+
+@[wp_expr_simp]
+theorem subst_pair {x v e₁ e₂} :
+  Exp.subst (.named x) v (.pair e₁ e₂) = (.pair (e₁.subst (.named x) v) (e₂.subst (.named x) v)) :=
+  by simp [Exp.subst, Exp.substStr]
+
+@[wp_expr_simp]
+theorem subst_fst {x v e} :
+  Exp.subst (.named x) v (.fst e) = (.fst (e.subst (.named x) v)) :=
+  by simp [Exp.subst, Exp.substStr]
+
+@[wp_expr_simp]
+theorem subst_snd {x v e} :
+  Exp.subst (.named x) v (.snd e) = (.snd (e.subst (.named x) v)) :=
+  by simp [Exp.subst, Exp.substStr]
+
+@[wp_expr_simp]
+theorem subst_injL {x v e} :
+  Exp.subst (.named x) v (.injL e) = (.injL (e.subst (.named x) v)) :=
+  by simp [Exp.subst, Exp.substStr]
+
+@[wp_expr_simp]
+theorem subst_injR {x v e} :
+  Exp.subst (.named x) v (.injR e) = (.injR (e.subst (.named x) v)) :=
+  by simp [Exp.subst, Exp.substStr]
+
+@[wp_expr_simp]
+theorem subst_allocN {x v e₁ e₂} :
+  Exp.subst (.named x) v (.allocN e₁ e₂) = (.allocN (e₁.subst (.named x) v) (e₂.subst (.named x) v)) :=
+  by simp [Exp.subst, Exp.substStr]
+
+@[wp_expr_simp]
+theorem subst_free {x v e} :
+  Exp.subst (.named x) v (.free e) = (.free (e.subst (.named x) v)) :=
+  by simp [Exp.subst, Exp.substStr]
+
+@[wp_expr_simp]
+theorem subst_load {x v e} :
+  Exp.subst (.named x) v (.load e) = (.load (e.subst (.named x) v)) :=
+  by simp [Exp.subst, Exp.substStr]
+
+@[wp_expr_simp]
+theorem subst_store {x v e₁ e₂} :
+  Exp.subst (.named x) v (.store e₁ e₂) = (.store (e₁.subst (.named x) v) (e₂.subst (.named x) v)) :=
+  by simp [Exp.subst, Exp.substStr]
+
+@[wp_expr_simp]
+theorem subst_cmpXchg {x v e₀ e₁ e₂} :
+  Exp.subst (.named x) v (.cmpXchg e₀ e₁ e₂) = (.cmpXchg (e₀.subst (.named x) v) (e₁.subst (.named x) v) (e₂.subst (.named x) v)) :=
+  by simp [Exp.subst, Exp.substStr]
+
+@[wp_expr_simp]
+theorem subst_xchg {x v e₁ e₂} :
+  Exp.subst (.named x) v (.xchg e₁ e₂) = (.xchg (e₁.subst (.named x) v) (e₂.subst (.named x) v)) :=
+  by simp [Exp.subst, Exp.substStr]
+
+@[wp_expr_simp]
+theorem subst_faa {x v e₁ e₂} :
+  Exp.subst (.named x) v (.faa e₁ e₂) = (.faa (e₁.subst (.named x) v) (e₂.subst (.named x) v)) :=
+  by simp [Exp.subst, Exp.substStr]
+
+@[wp_expr_simp]
+theorem subst_fork {x v e} :
+  Exp.subst (.named x) v (.fork e) = (.fork (e.subst (.named x) v)) :=
+  by simp [Exp.subst, Exp.substStr]
+
+@[wp_expr_simp]
+theorem subst_newProph {x v} :
+  Exp.subst (.named x) v .newProph = .newProph :=
+  by simp [Exp.subst, Exp.substStr]
+
+@[wp_expr_simp]
+theorem subst_resolve {x v e₀ e₁ e₂} :
+  Exp.subst (.named x) v (.resolve e₀ e₁ e₂) = (.resolve (e₀.subst (.named x) v) (e₁.subst (.named x) v) (e₂.subst (.named x) v)) :=
+  by simp [Exp.subst, Exp.substStr]
+
+simproc [wp_expr_simp] String.reduceEq_copy (( _ : String) = _) := String.reduceEq
+simproc [wp_expr_simp] reduceCtorEq_copy (_ = _) := reduceCtorEq
+attribute [wp_expr_simp] ne_eq not_false_eq_true Binder.named.injEq _root_.or_true _root_.true_or
+
+end wp_expr_simp
+
+
 public structure WpGoal where
   {u : Level}
   {prop : Q(Type u)}
@@ -82,7 +216,7 @@ public meta def iWpValueHead {u}
   (_hprop : $prop =Q IProp $GF := ⟨⟩)
   (_hbi : $bi =Q UPred.instBIUPred := ⟨⟩)
   (_hwp : $κ =Q wp.def := ⟨⟩) :
-    ProofModeM (Option Q($ehyps ⊢ Wp.wp $s $E $e $Φ)) := (do
+    ProofModeM (Option Q($ehyps ⊢ Wp.wp $s $E $e $Φ)) := do
   let ~q(ProgramLogic.ToVal.ofVal $v) := e
     | return none
   have goal : Q(IProp $GF) := Expr.headBeta q($Φ $v)
@@ -100,13 +234,66 @@ public meta def iWpValueHead {u}
       return some q(tac_wp_value_nofupd (s:=$s) (E:=$E) $pf)
 
   let pf ← addBIGoal hyps q(iprop(|={$E}=> $goal))
-  return some q(tac_wp_value (s:=$s) $pf))
+  return some q(tac_wp_value (s:=$s) $pf)
 
 elab "wp_value_head" : tactic =>
   ProofModeM.runTacticWp fun mvar {bi, hyps, ι, s, E, e, Φ, hbi, ..} => do
     have : $bi =Q UPred.instBIUPred := hbi
     let some pf ← iWpValueHead hyps ι q(wp.def) s E e Φ
       | throwTacticEx `wp_value_head mvar s!"{e} is not a value"
+    mvar.assign pf
+
+public meta def iWpExprSimp (e : Q(Exp)) :
+    ProofModeM ((e' : Q(Exp)) × Q($e = $e')) := do
+  let some ext ← getSimpExtension? `wp_expr_simp
+    | throwError "Cannot find `wp_expr_simp` attribute"
+  let some procext ← Simp.getSimprocExtension? `wp_expr_simp
+    | throwError "Cannot find `wp_expr_simp` attribute"
+
+  let theorems ← ext.getTheorems
+  let procs ← procext.getSimprocs
+  let simpctx := ← Simp.mkContext (simpTheorems := #[theorems])
+  let ⟨res, _⟩ ← Meta.simp e simpctx (simprocs:=#[procs])
+  return ⟨res.expr, ← res.getProof' e⟩
+
+public theorem tac_wp_expr_simp [ι : IrisGS_gen hlc Exp GF] {Δ} {s : Stuckness} {E : CoPset} {e e' : Exp} {Φ : Val → IProp GF}
+  (h : Δ ⊢ WP e' @ s ; E {{ Φ }})
+  (heq : e = e') :
+  (Δ ⊢ WP e @ s ; E {{ Φ }}) := by simp [*]
+
+elab "wp_expr_simp" : tactic =>
+  ProofModeM.runTacticWp fun mvar {hyps, s, E, e, Φ, ..} => do
+    let ⟨e', pfeq⟩ ← iWpExprSimp e
+    let pf ← addBIGoal hyps q(Wp.wp $s $E $e' $Φ)
+    mvar.assign q(tac_wp_expr_simp $pf $pfeq)
+
+public meta def iWpFinish {u}
+  {GF : Q(BundledGFunctors.{0, 0, 0})}
+  {hlc : Q(HasLC)}
+  {prop : Q(Type u)}
+  {bi : Q(BI $prop)}
+  {ehyps : Q($prop)}
+  (hyps : Hyps bi ehyps)
+  (ι : Q(IrisGS_gen $hlc Exp $GF))
+  (κ : Q(Wp $prop Exp Val Stuckness))
+  (s : Q(Stuckness))
+  (E : Q(CoPset))
+  (e : Q(Exp))
+  (Φ : Q(Val → $prop))
+
+  (_hu : QuotedLevelDefEq u 0 := ⟨⟩)
+  (_hprop : $prop =Q IProp $GF := ⟨⟩)
+  (_hbi : $bi =Q UPred.instBIUPred := ⟨⟩)
+  (_hwp : $κ =Q wp.def := ⟨⟩) :
+    ProofModeM (Q($ehyps ⊢ Wp.wp $s $E $e $Φ)) := do
+  let ⟨e', pfeq⟩ ← iWpExprSimp e
+  let nextPf ← (← iWpValueHead hyps ι q(wp.def) s E e' Φ).getDM
+      (addBIGoal hyps q(Wp.wp $s $E $e' $Φ))
+  return q(tac_wp_expr_simp $nextPf $pfeq)
+
+elab "wp_finish" : tactic =>
+  ProofModeM.runTacticWp fun mvar {hyps, ι, s, E, e, Φ, ..} => do
+    let pf ← iWpFinish hyps ι q(wp.def) s E e Φ
     mvar.assign pf
 
 public theorem tac_wp_bind [ι : IrisGS_gen hlc Exp GF] {Δ} {s : Stuckness} {E : CoPset} {K : List ECtxItem} {e' : Exp} {Φ : Val → IProp GF}
@@ -169,8 +356,7 @@ elab "wp_pure " colGt ppSpace focus:hl_exp : tactic =>
 
     let ⟨inner, .up _⟩ ← HeapLang.fillQ K e₂
 
-    let nextPf ← (← iWpValueHead hyps' ι q(wp.def) s E inner Φ).getDM
-      (addBIGoal hyps' q(Wp.wp $s $E $inner $Φ))
+    let nextPf ← iWpFinish hyps' ι q(wp.def) s E inner Φ
 
     let HΦ ← iSolveSidecondition q($φ) (failOnUnsolved := false)
 
@@ -180,6 +366,8 @@ elab "wp_pure " colGt ppSpace focus:hl_exp : tactic =>
 
 macro "wp_pure" : tactic => `(tactic| wp_pure _)
 macro "wp_pures" : tactic => `(tactic| repeat wp_pure)
+
+macro "wp_rec" : tactic => `(tactic | (iapply $(mkIdent `wp_rec):ident; rfl; imodintro; wp_finish))
 
 initialize registerTraceClass `wp_bind
 initialize registerTraceClass `wp_pure
